Attempt at proving the compatibility lemma for Apply * TODO: Finish the proof. If I can prove the compatibility lemmas for Var and LamAbs 	as well, then we can reasonably sure that this approach with step-indexed 	logical relations works!

src/Language/PlutusIR/Semantics/SemanticEquivalence/Def.v
@@ -7,7 +7,7 @@ Require Import PlutusCert.Language.PlutusIR.Semantics.Dynamic.
 Require Import Arith.
 
 
-Definition terminates := fun t k => exists v j, j < k /\ t =[j]=> v.
+Definition terminates := fun t k => exists v j, t =[j]=> v /\ j < k.
 
 Lemma e : forall i j k,
 i < k ->
@@ -23,30 +23,30 @@ Equations? R (k : nat ) (T : Ty) (t1 t2 : Term) : Prop by wf k :=
     emptyContext |-+ t1 : T /\
     emptyContext |-+ t2 : T /\
     forall v1 j1,
-      forall (Hj1 : j1 < k),
+      forall (Hlt_j1 : j1 < k),
       t1 =[j1]=> v1 ->
       exists v2 j2,
         t2 =[j2]=> v2 /\
           match T with
           | Ty_Forall X K T0 => 
-              forall t0_1 t0_2 T' j,
-                forall (Hj : j < k - j1),
+              forall t0_1 t0_2 T' k',
+                forall (Hlt_k' : k' < k - j1),
                 v1 = TyAbs X K t0_1 ->
                 v2 = TyAbs X K t0_2 ->
                 emptyContext |-* T' : K ->
-                R j (beta_reduce (substituteT X T' T0)) v1 v2
+                R k' (beta_reduce (substituteT X T' T0)) v1 v2
           | Ty_Fun T1 T2 => 
-              forall s1 s2 j,
-                forall (Hj : j < k - j1),
-                R j T1 s1 s2 ->
-                R j T2 (Apply v1 s1) (Apply v2 s2)
+              forall s1 s2 k',
+                forall (Hlt_k' : k' < k - j1),
+                R k' T1 s1 s2 ->
+                R k' T2 (Apply v1 s1) (Apply v2 s2)
           | Ty_Builtin st => 
               v1 = v2
           | Ty_IFix F T0 => 
-              forall K j,
-                forall (Hj : j < k - j1),
+              forall K k',
+                forall (Hlt_k' : k' < k - j1),
                 emptyContext |-* T0 : K ->
-                R j (beta_reduce (unwrapIFix F K T0)) v1 v2
+                R k' (beta_reduce (unwrapIFix F K T0)) v1 v2
           | _ => False (* Ty_Lam, Ty_Abs and Ty_Var should not occur *)
           end.
 Proof. all: try solve [eapply e; eauto]. Qed.
@@ -69,7 +69,7 @@ Proof. intros. destruct (R_typable_empty _ _ _ _ H). assumption. Qed.
 Lemma R_evaluable : forall k T t1 t2,
     terminates t1 k ->
     R k T t1 t2 ->
-    exists v1 v2 j1 j2, t1 =[j1]=> v1 /\ t2 =[j2]=> v2.
+    exists v1 v2 j1 j2, j1 < k /\ t1 =[j1]=> v1 /\ t2 =[j2]=> v2.
 Proof. intros. destruct H. destruct H. destruct H. autorewrite with R in H0.
   destruct T; destruct H0 as [_ [_ [v2 [j2 [Hev2 _]]]]]; eauto; 
     try solve [eexists; eexists; eexists; eexists; eauto].
@@ -78,19 +78,20 @@ Qed.
 Lemma R_evaluable_1 : forall k T t1 t2,
     terminates t1 k ->
     R k T t1 t2 ->
-    exists v1 j1, t1 =[j1]=> v1.
-Proof. intros. destruct (R_evaluable _ _ _ _ H H0) as [v1 [_ [j1 [_ [Hev1 _]]]]]; eauto. Qed.
+    exists v1 j1, j1 < k /\ t1 =[j1]=> v1.
+Proof. intros. destruct (R_evaluable _ _ _ _ H H0) as [v1 [_ [j1 [_ [Hlt1 [Hev1 _]]]]]]; eauto. Qed.
 
 Lemma R_evaluable_2 : forall k T t1 t2,
     terminates t1 k ->
     R k T t1 t2 ->
     exists v2 j2, t2 =[j2]=> v2.
-Proof. intros. destruct (R_evaluable _ _ _ _ H H0) as [_ [v2 [_ [j2 [_ Hev2]]]]]; eauto. Qed.
+Proof. intros. destruct (R_evaluable _ _ _ _ H H0) as [_ [v2 [_ [j2 [_ [_ Hev2]]]]]]; eauto. Qed.
 
 Lemma R_syntactic_equality : forall k st t1 t2,
     terminates t1 k ->
     R k (Ty_Builtin st) t1 t2 ->
     exists v1 v2 j1 j2,
+      j1 < k /\
       t1 =[j1]=> v1 /\
       t2 =[j2]=> v2 /\
       v1 = v2.
@@ -103,26 +104,64 @@ Lemma R_functional_extensionality : forall k T1 T2 t1 t2,
     terminates t1 k ->
     R k (Ty_Fun T1 T2) t1 t2 ->
     exists v1 v2 j1 j2,
+      j1 < k /\
       t1 =[j1]=> v1 /\
       t2 =[j2]=> v2 /\
-      (forall s1 s2 j,
-        j < k - j1 ->
-        R j T1 s1 s2 ->
-        R j T2 (Apply v1 s1) (Apply v2 s2)).
+      (forall s1 s2 k',
+        k' < k - j1 ->
+        R k' T1 s1 s2 ->
+        R k' T2 (Apply v1 s1) (Apply v2 s2)).
 Proof. 
-  intros. destruct H. destruct H. destruct H.
-  autorewrite with R in H0.
-  destruct H0.
-  destruct H2.
-  edestruct H3; eauto.
-  destruct H4.
-  destruct H4.
-  exists x.
-  exists x1.
-  exists x0.
-  exists x2.
-  split; eauto.
+  intros k T1 T2 t1 t2 Hterm R. 
+  destruct Hterm as [v1 [j1 [Hev1 Hlt_j1]]].
+  autorewrite with R in R.
+  destruct R as [_ [_ [v2 [j2 [Hev_t2 Hfe]]]]]; eauto.
+  exists v1, v2, j1, j2. 
+  auto.
 Qed.
+
+Lemma R_unwrap : forall k F T t1 t2,
+    terminates t1 k ->
+    R k (Ty_IFix F T) t1 t2 ->
+    exists v1 v2 j1 j2,
+      j1 < k /\
+      t1 =[j1]=> v1 /\
+      t2 =[j2]=> v2 /\
+      (forall K k',
+        k' < k - j1 ->
+        emptyContext |-* T : K ->
+        R k' (beta_reduce (unwrapIFix F K T)) v1 v2).
+Proof.
+  intros k F T t1 t2 Hterm R. 
+  destruct Hterm as [v1 [j1 [Hev1 Hlt_j1]]].
+  autorewrite with R in R.
+  destruct R as [_ [_ [v2 [j2 [Hev_t2 Hunwrap]]]]]; eauto.
+  exists v1, v2, j1, j2.
+  auto.
+Qed.
+
+Lemma R_instantiational_extensionality : forall k X K T t1 t2,
+    terminates t1 k ->
+    R k (Ty_Forall X K T) t1 t2 ->
+    exists v1 v2 j1 j2,
+      j1 < k /\
+      t1 =[j1]=> v1 /\
+      t2 =[j2]=> v2 /\
+      (forall t0_1 t0_2 T' k',
+        k' < k - j1 ->
+        v1 = TyAbs X K t0_1 ->
+        v2 = TyAbs X K t0_2 ->
+        emptyContext |-* T' : K ->
+        R k' (beta_reduce (substituteT X T' T)) v1 v2).
+Proof.
+  intros k X K T t1 t2 Hterm R. 
+  destruct Hterm as [v1 [j1 [Hev1 Hlt_j1]]].
+  autorewrite with R in R.
+  destruct R as [_ [_ [v2 [j2 [Hev_t2 Hie]]]]]; eauto.
+  exists v1, v2, j1, j2.
+  auto.
+Qed.
+
 
 Lemma R_impossible_type : forall k t1 t2,
     terminates t1 k ->
@@ -142,8 +181,8 @@ Proof.
   intros. destruct H.
   destruct H.
   destruct H.
-  apply PeanoNat.Nat.nlt_0_r in H.
-  destruct H.
+  apply PeanoNat.Nat.nlt_0_r in H0.
+  destruct H0.
 Qed.
 
 Lemma R_nontermination : forall k T t1 t2,
