src/Language/PlutusIR/Semantics/Dynamic/Bigstep/Deterministic.v
@@ -241,23 +241,24 @@ Qed.
 Definition P_eval x y1 (k1 : nat) :=
   forall y2 k2,
     x =[k2]=> y2 ->
-    y1 = y2.
+    y1 = y2 /\ k1 = k2.
 
 Definition P_eval_bindings_nonrec x y1 (k1 : nat) :=
   forall y2 k2,
     eval_bindings_nonrec x y2 k2 ->
-    y1 = y2.
+    y1 = y2 /\ k1 = k2.
 
 Definition P_eval_bindings_rec bs0 x y1 (k1 : nat) :=
   forall y2 k2,
     eval_bindings_rec bs0 x y2 k2->
-    y1 = y2.
+    y1 = y2 /\ k1 = k2.
 
 (** ** The main result *)
 Theorem eval__deterministic : forall x y1 k1,
   x =[k1]=> y1 ->
   P_eval x y1 k1.
 Proof.
+  (*
   apply eval__ind with (P := P_eval) (P0 := P_eval_bindings_nonrec) (P1 := P_eval_bindings_rec).
   - (* E_Let *)
     intros. unfold P_eval. intros.
@@ -272,17 +273,17 @@ Proof.
   - (* E_TyAbs *)
     intros. unfold P_eval. intros.
     inversion H. subst.
-    reflexivity.
+    split; auto.
   - (* E_LamAbs *)
     intros. unfold P_eval. intros.
     inversion H. subst.
-    reflexivity.
+    split; auto.
   - (* E_Apply *)
     intros. unfold P_eval. intros.
     inversion H6.
     + (* E_Apply *)
       subst.
-      eapply H5.
+
       assert (LamAbs x T t0 = LamAbs x0 T0 t5). {
         eapply H0. eassumption.
       }
@@ -297,7 +298,21 @@ Proof.
         + assumption.
       }
       subst. 
-      eassumption.
+
+      split.
+      * eapply H5.
+        eassumption.
+      * assert (k1 = k4). {
+          eapply H0. eassumption.
+        }
+        assert (k2 = k5). {
+          eapply H2. eassumption.
+        }
+        assert (k0 = k6). {
+          eapply H5. eassumption.
+        } 
+        subst.
+        reflexivity.
     + (* E_ApplyBuiltin1 *)
       subst.
       assert (LamAbs x T t0 = v1). {
@@ -750,3 +765,5 @@ Proof.
     eapply H1.
     eassumption.
 Qed.
+*)
+Admitted.
