src/Language/PlutusIR/Semantics/SemanticEquivalence/CompatibilityLemmas/Apply.v
@@ -1,0 +1,76 @@
+Require Import PlutusCert.Language.PlutusIR.
+Import NamedTerm.
+Require Import PlutusCert.Language.PlutusIR.Semantics.Dynamic.
+Require Import PlutusCert.Language.PlutusIR.Semantics.Static.
+Require Import PlutusCert.Language.PlutusIR.Semantics.Static.Implementations.Named.
+Require Import PlutusCert.Language.PlutusIR.Semantics.Static.Implementations.Named.ContextInvariance.
+Require Import PlutusCert.Language.PlutusIR.Semantics.TypeSafety.Preservation.
+Require Import PlutusCert.Language.PlutusIR.Semantics.TypeSafety.SubstitutionPreservesTyping.
+Require Import PlutusCert.Language.PlutusIR.Semantics.SemanticEquivalence.Def.
+Require Import PlutusCert.Language.PlutusIR.Semantics.SemanticEquivalence.Monotonicity.
+Require Import PlutusCert.Language.PlutusIR.Semantics.SemanticEquivalence.ReductionInvariance.
+
+Require Import Arith.
+
+Lemma termination_congr_Apply1 : forall t1 t2 k,
+  terminates (Apply t1 t2) k ->
+  terminates t1 k.
+Proof.
+  intros.
+  destruct H as [v0 [j [Hlt_j]]].
+  inversion Hlt_j.
+  - subst.
+    exists (LamAbs x T t4).
+    exists k1.
+    split; auto.
+    apply skip.
+Admitted.
+
+Lemma termination_congr_Apply2 : forall t1 t2 k,
+  terminates (Apply t1 t2) k ->
+  terminates t2 k.
+Proof. Admitted.
+
+Lemma R_compatibility_Apply : forall k T1 T2 t1_1 t1_2 t2_1 t2_2,
+    (terminates (Apply t1_1 t1_2) k \/ ~ terminates (Apply t2_1 t2_2) k) ->
+    R k (Ty_Fun T1 T2) t1_1 t2_1 ->
+    R k T1 t1_2 t2_2 ->
+    R k T2 (Apply t1_1 t1_2) (Apply t2_1 t2_2).
+Proof.
+  intros k T1 T2 t1_1 t1_2 t2_1 t2_2 Hterm R1 R2.
+
+  assert (Htyp1 : emptyContext |-+ (Apply t1_1 t1_2) : T2). {
+    apply T_Apply with T1.
+    - eapply R_typable_empty_1; eauto.
+    - eapply R_typable_empty_1; eauto.
+  } 
+  assert (Htyp2 : emptyContext |-+ (Apply t2_1 t2_2) : T2). {
+    apply T_Apply with T1.
+    - eapply R_typable_empty_2; eauto.
+    - eapply R_typable_empty_2; eauto.
+  }
+
+  autorewrite with R.
+  
+  destruct T2.
+  - (* Ty_Var S *)
+    split; auto. split; auto.
+
+    intros v1_0 j1 Hlt_j1 Hev1. 
+
+    assert (Hterm1: terminates (Apply t1_1 t1_2) k). {
+      exists v1_0, j1. auto.
+    }
+    assert (Hterm_t1_1 : terminates t1_1 k). {
+      inversion Hev1; subst; eapply termination_congr_Apply1; eauto.
+    }
+    assert (Hterm_t1_2 : terminates t1_2 k). {
+      inversion Hev1; subst; eapply termination_congr_Apply2; eauto.
+    }
+
+    apply R_functional_extensionality in R1 as temp; eauto.
+    destruct temp as [v1_1 [v2_1 [j1_1 [j2_1 [Hlt1_1 [Hev1_1 [Hev2_1 Hfe]]]]]]].
+    destruct k. {
+      apply R_impossible_k in R1; eauto. destruct R1.
+    }
+Abort.
