src/Language/PlutusIR/Semantics/SemanticEquivalence/ReductionInvariance.v
@@ -1,0 +1,284 @@
+Require Import PlutusCert.Language.PlutusIR.
+Import NamedTerm.
+Require Import PlutusCert.Language.PlutusIR.Semantics.Static.
+Require Import PlutusCert.Language.PlutusIR.Semantics.Static.Implementations.Named.
+Require Import PlutusCert.Language.PlutusIR.Semantics.Dynamic.
+Require Import PlutusCert.Language.PlutusIR.Semantics.TypeSafety.Preservation.
+Require Import PlutusCert.Language.PlutusIR.Semantics.SemanticEquivalence.Def.
+
+Require Import Arith.
+
+Lemma eval_preserves_termination : forall t v k j,
+    terminates t k ->
+    t =[j]=> v ->
+    j < k ->
+    terminates v k.
+Proof. intros. exists v, 0.
+  split.
+  - apply eval_value. eapply eval_to_value. eassumption.
+  - destruct (Nat.eq_0_gt_0_cases k).
+    + subst. apply Nat.nlt_0_r in H1. destruct H1.
+    + assumption.
+Qed.
+
+Lemma e : forall j k i,
+    0 < k ->
+    j < k - 0 ->
+    j < k - i.
+Proof. Admitted.
+
+(** * Evaluation of terms preserves [R] (forward preservation) *)
+
+(** ** Evaluation of the first related term preserves [R] *)
+
+Lemma eval_preserves_R_left : forall k T t1 j1 v1 t2,
+    terminates t1 k ->
+    t1 =[j1]=> v1 ->
+    j1 < k ->
+    R k T t1 t2 ->
+    R k T v1 t2.
+Proof.
+  intros k T t1 j1 v1 t2 Hterm_t1 Hev_t1 Hlt R.
+
+  assert (emptyContext |-+ t1 : T) by eauto using R_typable_empty_1.
+  assert (emptyContext |-+ t2 : T) by eauto using R_typable_empty_2.
+  assert (emptyContext |-+ v1 : T) by eauto using preservation.
+
+  autorewrite with R.
+  destruct T.
+  - apply R_impossible_type in R; auto. destruct R.
+  - apply R_functional_extensionality in R as Hfe; auto.
+    destruct Hfe as [v1' [v2 [j1' [j2 [Hlt_j1' [Hev_t1' [Hev_t2 Hfe]]]]]]].
+  
+    split; auto. split; auto.
+    intros v0 j0 Hlt_j0 Hev_v1.
+    exists v2, j2. split; auto.
+    
+    intros s1 s2 k' Hlt_k' R'. 
+    assert (v1' = v1 /\ j1' = j1) by (eapply eval__deterministic; eauto).
+    destruct H2. subst.
+    apply eval_to_value in Hev_t1 as Hval_v1.
+    apply eval_value in Hval_v1.
+    unfold P_value in Hval_v1.
+    assert (v0 = v1 /\ j0 = 0) by (eapply eval__deterministic; eauto).
+    destruct H2. subst. 
+    apply Hfe.
+    + eapply e; eauto.
+    + assumption.
+  - (* Ty_IFix *)
+    apply R_unwrap in R as Hunwr; auto.
+    destruct Hunwr as [v1' [v2 [j1' [j2 [Hlt_j1' [Hev_t1' [Hev_t2 Hunwr]]]]]]].
+    
+    split; auto. split; auto.
+    intros v0 j0 Hlt_j0 Hev_v1.
+    exists v2, j2. split; auto.
+
+    intros K k' Hlt_k' Hkind_T2.
+    assert (v1' = v1 /\ j1' = j1) by (eapply eval__deterministic; eauto).
+    destruct H2. subst.
+    apply eval_to_value in Hev_t1 as Hval_v1.
+    apply eval_value in Hval_v1 as Hev_v1'.
+    unfold P_value in Hev_v1'.
+    assert (v0 = v1 /\ j0 = 0) by (eapply eval__deterministic; eauto).
+    destruct H2. subst.
+    apply Hunwr.
+    + eapply e; eauto.
+    + assumption.
+  - (* Ty_Forall *)
+    apply R_instantiational_extensionality in R as Hie; auto.
+    destruct Hie as [v1' [v2 [j1' [j2 [Hlt_j1' [Hev_t1' [Hev_t2 Hie]]]]]]].
+
+    split; auto. split; auto.
+    intros v0 j0 Hlt_j0 Hev_v1.
+    exists v2, j2. split; auto.
+
+    intros t0_1 t0_2 T' k' Hlt_k' Heq1 Heq2 Hkind_T'.
+    assert (v1' = v1 /\ j1' = j1) by (eapply eval__deterministic; eauto).
+    destruct H2. subst.
+    apply eval_to_value in Hev_t1 as Hval_v1.
+    apply eval_value in Hval_v1 as Hev_v1'.
+    unfold P_value in Hev_v1'.
+    assert (TyAbs s k0 t0_1 = v1 /\ j0 = 0) by (eapply eval__deterministic; eauto).
+    destruct H2. subst.
+    eapply Hie.
+    + apply e; eauto.
+    + reflexivity.
+    + reflexivity.
+    + assumption.
+  - (* Ty_Builtin *)
+    apply R_syntactic_equality in R as Hse; auto.
+    destruct Hse as [v1' [v2 [j1' [j2 [Hlt_j1' [Hev_t1' [Hev_t2 Hse]]]]]]].
+    subst.
+
+    split; auto. split; auto.
+    intros v0 j0 Hlt_j0 Hev_v1.
+    exists v2, j2. split; auto.
+
+    assert (v2 = v1 /\ j1' = j1) by (eapply eval__deterministic; eauto).
+    destruct H2. subst.
+    apply eval_to_value in Hev_t1 as Hval_v1.
+    apply eval_value in Hval_v1 as Hev_v1'.
+    unfold P_value in Hev_v1'.
+    assert (v0 = v1 /\ j0 = 0) by (eapply eval__deterministic; eauto).
+    destruct H2. subst.
+    reflexivity.
+  - (* Ty_Lam *)
+    apply R_impossible_type in R; auto. destruct R.
+  - (* Ty_App *)
+    apply R_impossible_type in R; auto. destruct R.
+Qed.
+
+(** ** Evaluation of the second related term preserves [R] *)
+
+Lemma eval_preserves_R_right : forall k T t1 t2 j2 v2,
+    terminates t1 k ->
+    t2 =[j2]=> v2 ->
+    R k T t1 t2 ->
+    R k T t1 v2.
+Proof. 
+  intros k T t1 t2 j2 v2 Hterm_t1 Hev_t2 R.
+
+  assert (emptyContext |-+ t1 : T) by eauto using R_typable_empty_1.
+  assert (emptyContext |-+ t2 : T) by eauto using R_typable_empty_2.
+  assert (emptyContext |-+ v2 : T) by eauto using preservation.
+
+  autorewrite with R.
+  destruct T.
+  - apply R_impossible_type in R; auto. destruct R.
+  - apply R_functional_extensionality in R as Hfe; auto.
+    destruct Hfe as [v1 [v2' [j1 [j2' [Hlt_j1 [Hev_t1 [Hev_t2' Hfe]]]]]]].
+  
+    split; auto. split; auto.
+    intros v1' j1' Hlt_j1' Hev_t1'.
+
+    assert (v2' = v2 /\ j2' = j2) by (eapply eval__deterministic; eauto).
+    destruct H2. subst.
+    apply eval_to_value in Hev_t2 as Hval_v2.
+    apply eval_value in Hval_v2 as Hev_v2.
+    unfold P_value in Hev_v2.
+
+    exists v2, 0. split; auto.
+
+    assert (v1' = v1 /\ j1' = j1) by (eapply eval__deterministic; eauto).
+    destruct H2. subst.
+
+    apply Hfe.
+  - (* Ty_IFix *)
+    apply R_unwrap in R as Hunwr; auto.
+    destruct Hunwr as [v1 [v2' [j1 [j2' [Hlt_j1 [Hev_t1 [Hev_t2' Hunwr]]]]]]].
+
+    split; auto. split; auto.
+    intros v1' j1' Hlt_j1' Hev_t1'.
+
+    assert (v2' = v2 /\ j2' = j2) by (eapply eval__deterministic; eauto).
+    destruct H2. subst.
+    apply eval_to_value in Hev_t2 as Hval_v2.
+    apply eval_value in Hval_v2 as Hev_v2.
+    unfold P_value in Hev_v2.
+
+    exists v2, 0. split; auto.
+
+    assert (v1' = v1 /\ j1' = j1) by (eapply eval__deterministic; eauto).
+    destruct H2. subst.
+
+    apply Hunwr.
+  - (* Ty_Forall *)
+    apply R_instantiational_extensionality in R as Hie; auto.
+    destruct Hie as [v1 [v2' [j1 [j2' [Hlt_j1 [Hev_t1 [Hev_t2' Hie]]]]]]].
+
+    split; auto. split; auto.
+    intros v1' j1' Hlt_j1' Hev_t1'.
+
+    assert (v2' = v2 /\ j2' = j2) by (eapply eval__deterministic; eauto).
+    destruct H2. subst.
+    apply eval_to_value in Hev_t2 as Hval_v2.
+    apply eval_value in Hval_v2 as Hev_v2.
+    unfold P_value in Hev_v2.
+
+    exists v2, 0. split; auto.
+
+    assert (v1' = v1 /\ j1' = j1) by (eapply eval__deterministic; eauto).
+    destruct H2. subst.
+
+    apply Hie.
+  - (* Ty_Builtin *)
+    apply R_syntactic_equality in R as Hse; auto.
+    destruct Hse as [v1 [v2' [j1 [j2' [Hlt_j1 [Hev_t1 [Hev_t2' Hse]]]]]]].
+
+    split; auto. split; auto.
+    intros v1' j1' Hlt_j1' Hev_t1'.
+
+    assert (v2' = v2 /\ j2' = j2) by (eapply eval__deterministic; eauto).
+    destruct H2. subst.
+    apply eval_to_value in Hev_t2 as Hval_v2.
+    apply eval_value in Hval_v2 as Hev_v2.
+    unfold P_value in Hev_v2.
+
+    exists v2, 0. split; auto.
+
+    eapply eval__deterministic; eauto.
+  - (* Ty_Lam *)
+    apply R_impossible_type in R; auto. destruct R.
+  - (* Ty_App *)
+    apply R_impossible_type in R; auto. destruct R.
+Qed.
+
+(** ** Evaluation of both related terms preserves [R] *)
+
+Lemma eval_preserves_R : forall k T t1 j1 v1 t2 j2 v2,
+    terminates t1 k ->
+    t1 =[j1]=> v1 ->
+    j1 < k ->
+    t2 =[j2]=> v2 ->
+    R k T t1 t2 ->
+    R k T v1 v2.
+Proof.
+  intros k T t1 j1 v1 t2 j2 v2 Hterm1 Hev1 Hlt1 Hev2 R.
+  eapply eval_preserves_R_left; eauto.
+  eapply eval_preserves_R_right; eauto.
+Qed.
+
+
+
+(** * Evaluation of terms preserved [R] (backward preservation) *)
+
+(** ** Evaluation of the first related term preserved [R] *)
+
+Lemma eval_preserved_R_left : forall k T t1 j1 v1 t2,
+    emptyContext |-+ t1 : T ->
+    terminates t1 k ->
+    t1 =[j1]=> v1 ->
+    j1 < k ->
+    R k T v1 t2 ->
+    R k T t1 t2.
+Proof. Abort.
+
+(** ** Evaluation of the second related term preserved [R] *)
+
+Lemma eval_preserved_R_right : forall k T t1 t2 j2 v2,
+    emptyContext |-+ t2 : T ->
+    terminates t1 k ->
+    t2 =[j2]=> v2 ->
+    R k T t1 v2 ->
+    R k T t1 t2.
+Proof. Abort.
+
+(** ** Evaluation of the both related terms preserved [R] *)
+
+Lemma eval_preserved_R : forall k T t1 j1 v1 t2 j2 v2,
+    emptyContext |-+ t1 : T ->
+    emptyContext |-+ t2 : T ->
+    terminates t1 k ->
+    t1 =[j1]=> v1 ->
+    j1 < k ->
+    t2 =[j2]=> v2 ->
+    R k T v1 v2 ->
+    R k T t1 t2.
+Proof.
+  intros k T t1 j1 v1 t2 j2 v2 Htyp_t1 Htyp_t2 Hterm1 Hev1 Hlt1 Hev2 R.
+  (*
+  apply eval_preserved_R_left with v1; auto.
+  apply eval_preserved_R_right with v2; auto.
+  apply eval_preserves_termination with t1; auto.
+  *)
+Abort. 
